src/Norm.v
@@ -1,0 +1,269 @@
+Require Import
+  Coq.Unicode.Utf8
+  Coq.Lists.List
+  Coq.Logic.Classical
+  Ty
+  Exp
+  Sub
+  Sem
+  Eval.
+
+From Equations Require Import Equations.
+Set Equations With UIP.
+
+Generalizable All Variables.
+
+Import ListNotations.
+
+Definition normal_form {X : Type} (R : relation X) (t : X) : Prop :=
+  ¬ ∃ t', R t t'.
+
+Theorem value_is_nf {τ} (v : Exp [] τ) :
+  ValueP v → normal_form Step v.
+Proof.
+  intros.
+  unfold normal_form.
+  dependent induction v using Exp_rect';
+  inv H; intro; reduce.
+  - now inversion H.
+  - inv H.
+    apply Forall_app in H2.
+    reduce.
+    inv H0.
+    apply isplit in X; simpl in *; reduce.
+    now eapply n; eauto.
+  - now inversion H.
+Qed.
+
+Lemma substitution_reduces {τ ty} (e : Exp [ty] τ) v :
+  STmExp {|v|} e ≠ APP (LAM e) v.
+Proof.
+  intro.
+  dependent induction e; simpl in H; inv H.
+  - dependent elimination v; simp consSub in H1.
+    + induction v0; inv H1.
+      now intuition.
+    + now induction v; inv H1.
+  - admit.
+Admitted.
+
+(* A term never reduces to itself. *)
+Fixpoint Step_irr {τ} {x : Exp [] τ} : ¬ (x ---> x).
+Proof.
+  intro.
+  dependent induction x.
+  - now inv H.
+  - inv H.
+    clear -H4.
+    induction x2; inv H4.
+    now eapply IHx2_2; eauto.
+  - induction l.
+    + inv H.
+      destruct pre; simpl in *;
+      now inv H1.
+    + inv H.
+      destruct pre; simpl in *;
+      inv H1; inv H2.
+      * exact (Step_irr _ _ H4).
+      * apply app_inv_head in H0.
+        inv H0.
+        apply IHl.
+        constructor; auto.
+        now inv H3.
+  - now inv H.
+  - now inv H.
+  - now inv H.
+  - inv H.
+    + now eapply substitution_reduces; eauto.
+    + now eapply IHx1; eauto.
+    + now eapply IHx2; eauto.
+Qed.
+
+(* This injectivity theorem says that there is exactly one way to reduce terms
+   at any given step. *)
+Theorem Step_inj {τ} {x y z : Exp [] τ} :
+  x ---> y → x ---> z → y = z.
+Proof.
+  intros.
+  dependent induction x; intros; try solve [ now inv H ].
+  - now inv H; inv H0.
+  - admit.
+  - now inv H; inv H0.
+  - admit.
+Abort.
+
+Definition deterministic {X : Type} (R : relation X) :=
+  ∀ x y1 y2 : X, R x y1 → R x y2 → y1 = y2.
+
+Theorem step_deterministic τ :
+  deterministic (@Step τ).
+Proof.
+  repeat intro.
+  dependent induction x using Exp_rect'; try inv H.
+  - now inv H0.
+  - apply isplit in X; simpl in *; reduce.
+    now rewrite (Step_List_inv H0 H5).
+  - now inv H0.
+  - inv H0; auto.
+    + now inversion H3.
+    + apply value_is_nf in H3.
+      destruct H3.
+      now exists e2'.
+  - inv H0.
+    + now inversion H3.
+    + f_equal.
+      now eapply IHx1.
+    + apply value_is_nf in H4.
+      destruct H4.
+      now exists e1'.
+  - inv H0.
+    + apply value_is_nf in H2.
+      destruct H2.
+      now exists e2'.
+    + apply value_is_nf in H4.
+      destruct H4.
+      now exists e1'.
+    + f_equal.
+      now eapply IHx2.
+Qed.
+
+Theorem strong_progress {τ} (e : Exp [] τ) :
+  ValueP e ∨ ∃ e', e ---> e'.
+Proof.
+  dependent induction e using Exp_rect'.
+  - now left; constructor.
+  - right.
+    eexists e2.
+    now constructor.
+  - induction l; simpl in *.
+    + left.
+      now constructor.
+    + destruct X.
+      destruct (o _ eq_refl JMeq_refl).
+      * intuition.
+        ** left.
+           constructor.
+           inv H1.
+           now constructor.
+        ** right.
+           destruct H1.
+           inv H0.
+           exists (List (a :: pre ++ x' :: post)).
+           now apply ST_ListElem
+             with (pre:=a :: pre) (post:=post) (x:=x0) (x':=x'); auto.
+      * right.
+        destruct H.
+        exists (List (x :: l)).
+        now apply ST_ListElem
+          with (pre:=[]) (post:=l) (x:=a) (x':=x); auto.
+  - right.
+    exists (APP (LAM e2) e1).
+    now constructor.
+  - now inversion v.
+  - left.
+    now constructor.
+  - right.
+    destruct (IHe1 _ eq_refl JMeq_refl); clear IHe1.
+    + destruct (IHe2 _ eq_refl JMeq_refl); clear IHe2.
+      * dependent elimination e1; inv H.
+        exists (STmExp {| e2 |} e4).
+        now constructor.
+      * dependent elimination e1; inv H.
+        exists (APP (LAM e4) x).
+        constructor; auto.
+        now constructor.
+    + reduce.
+      destruct (IHe2 _ eq_refl JMeq_refl); clear IHe2.
+      * exists (APP x e2).
+        now constructor.
+      * reduce.
+        exists (APP x e2).
+        now constructor.
+Qed.
+
+Corollary nf_is_value τ (v : Exp [] τ) :
+  normal_form Step v → ValueP v.
+Proof.
+  intros.
+  destruct (strong_progress v); auto.
+  exfalso.
+  now apply H.
+Qed.
+
+Corollary nf_same_as_value τ (v : Exp [] τ) :
+  normal_form Step v ↔ ValueP v.
+Proof.
+  split.
+  - now apply nf_is_value.
+  - now apply value_is_nf.
+Qed.
+
+Inductive multi {X : Type} (R : relation X) : relation X :=
+  | multi_refl : ∀ (x : X), multi R x x
+  | multi_step : ∀ (x y z : X),
+      R x y →
+      multi R y z →
+      multi R x z.
+
+Notation " t '--->*' t' " := (multi Step t t') (at level 40).
+
+Theorem multi_R : ∀ (X : Type) (R : relation X) (x y : X),
+  R x y → (multi R) x y.
+Proof.
+  intros.
+  eapply multi_step; eauto.
+  now constructor.
+Qed.
+
+Theorem multi_trans : ∀ (X : Type) (R : relation X) (x y z : X),
+  multi R x y →
+  multi R y z →
+  multi R x z.
+Proof.
+  intros.
+  induction H; auto.
+  now eapply multi_step; eauto.
+Qed.
+
+Definition halts {τ} (e : Exp [] τ) : Prop :=
+  ∃ e', e --->* e' ∧ ValueP e'.
+
+Lemma value_halts {τ} (v : Exp [] τ) : ValueP v → halts v.
+Proof.
+  intros.
+  unfold halts.
+  now dependent induction H; eexists; split; constructor.
+Qed.
+
+Lemma step_preserves_halting {τ} (e e' : Exp [] τ) :
+  (e ---> e') → (halts e ↔ halts e').
+Proof.
+  intros.
+  unfold halts.
+  split.
+  - intros [e'' [H1 H2]].
+    destruct H1.
+    + apply value_is_nf in H2.
+      destruct H2.
+      now exists e'.
+    + rewrite (step_deterministic _ _ _ _ H H0).
+      now exists z.
+  - intros [e'0 [H1 H2]].
+    exists e'0.
+    split; auto.
+    now eapply multi_step; eauto.
+Qed.
+
+Definition normal_form_of {τ} (e e' : Exp [] τ) :=
+  (e --->* e' ∧ normal_form Step e').
+
+Theorem normal_forms_unique τ :
+  deterministic (normal_form_of (τ:=τ)).
+Proof.
+  unfold normal_form_of, normal_form.
+  repeat intro.
+  reduce.
+Admitted.
+
+Definition normalizing {X : Type} (R : relation X) :=
+  ∀ t, ∃ t', (multi R) t t' ∧ normal_form R t'.
